contrib/field/Field_Compl.v
@@ -18,26 +18,23 @@ Fixpoint appT [A:Type][l:(listT A)] : (listT A) -> (listT A) :=
   | (consT a l1) => (consT A a (appT A l1 m))
   end.
 
-Inductive Sprod [A:Type;B:Set] : Type :=
-  Spair : A -> B -> (Sprod A B).
+Inductive prodT [A,B:Type] : Type :=
+  pairT: A->B->(prodT A B).
 
 Definition assoc_2nd :=
 Fix assoc_2nd_rec
   {assoc_2nd_rec 
-   [A:Type;B:Set;eq_dec:(e1,e2:B){e1=e2}+{~e1=e2};lst:(listT (Sprod A B))]
+   [A:Type;B:Set;eq_dec:(e1,e2:B){e1=e2}+{~e1=e2};lst:(listT (prodT A B))]
    : B->A->A:=
   [key:B;default:A]
   Cases lst of
   | nilT => default
-  | (consT (Spair v e) l) =>
+  | (consT (pairT v e) l) =>
     (Cases (eq_dec e key) of
     | (left _) => v
     | (right _) => (assoc_2nd_rec A B eq_dec l key default)
     end)
   end}.
-
-Inductive prodT [A,B:Type] : Type :=
-  pairT: A->B->(prodT A B).
 
 Definition fstT [A,B:Type;c:(prodT A B)] :=
   Cases c of
